Typed equivalence relation on terms...

DeBruijnSSA/BinSyntax/Rewrite/Definitions.lean
@@ -14,12 +14,200 @@ def Term.WfD.subst₂ {Γ : Ctx α ε} {a b : Term φ}
   | ⟨1, _⟩ => hb
   | ⟨n + 2, h⟩ => var ⟨by simp at h; exact h, le_refl _⟩
 
-structure Region.HaveTrg (Γ : Ctx α ε) (L : LCtx α) (r r' : Region φ) where
+namespace Region
+
+structure HaveTrg (Γ : Ctx α ε) (L : LCtx α) (r r' : Region φ) where
   left : r.WfD Γ L
   right : r'.WfD Γ L
 
-inductive Region.WfD.Cong (P : Ctx α ε → LCtx α → Region φ → Region φ → Type _)
-  : Ctx α ε → LCtx α → Region φ → Region φ → Type _
+inductive WfD.CongD (P : Ctx α ε → LCtx α → Region φ → Region φ → Sort _)
+  : Ctx α ε → LCtx α → Region φ → Region φ → Sort _
+  | step : P Γ L r r' → CongD P Γ L r r'
+  | case_left : e.WfD Γ ⟨Ty.coprod A B, ⊥⟩ → CongD P (⟨A, ⊥⟩::Γ) L r r' → s.WfD (⟨B, ⊥⟩::Γ) L
+    → CongD P Γ L (Region.case e r s) (Region.case e r' s)
+  | case_right : e.WfD Γ ⟨Ty.coprod A B, ⊥⟩ → r.WfD (⟨A, ⊥⟩::Γ) L → CongD P (⟨B, ⊥⟩::Γ) L s s'
+    → CongD P Γ L (Region.case e r s) (Region.case e r s')
+  | let1 : e.WfD Γ ⟨A, e'⟩ → CongD P (⟨A, ⊥⟩::Γ) L r r'
+    → CongD P Γ L (Region.let1 e r) (Region.let1 e r')
+  | let2 : e.WfD Γ ⟨Ty.prod A B, e'⟩ → CongD P (⟨B, ⊥⟩::⟨A, ⊥⟩::Γ) L r r'
+    → CongD P Γ L (Region.let2 e r) (Region.let2 e r')
+  | cfg_entry (R : LCtx α) :
+    (hR : R.length = n) →
+    CongD P Γ (R ++ L) β β' →
+    (∀i : Fin n, (G i).WfD (⟨R.get (i.cast hR.symm), ⊥⟩::Γ) (R ++ L)) →
+    CongD P Γ L (Region.cfg β n G) (Region.cfg β' n G)
+  | cfg_block (R : LCtx α) :
+    (hR : R.length = n) →
+    β.WfD Γ (R ++ L) →
+    (hG : ∀i : Fin n, (G i).WfD (⟨R.get (i.cast hR.symm), ⊥⟩::Γ) (R ++ L)) →
+    (i : Fin n) →
+    CongD P (⟨R.get (i.cast hR.symm), ⊥⟩::Γ) (R ++ L) r r' →
+    CongD P Γ L (Region.cfg β n (Function.update G i r)) (Region.cfg β n (Function.update G i r'))
+
+def WfD.CongD.left {P : Ctx α ε → LCtx α → Region φ → Region φ → Sort _} {Γ L r r'}
+  (toLeft : ∀{Γ L r r'}, P Γ L r r' → r.WfD Γ L) : CongD P Γ L r r' → r.WfD Γ L
+  | step p => toLeft p
+  | case_left de pr ds => case de (pr.left toLeft) ds
+  | case_right de dr ps => case de dr (ps.left toLeft)
+  | let1 de pr => WfD.let1 de (pr.left toLeft)
+  | let2 de pr => WfD.let2 de (pr.left toLeft)
+  | cfg_entry R hR pβ dG => WfD.cfg _ R hR (pβ.left toLeft) dG
+  | cfg_block R hR dβ dG i pr => WfD.cfg _ R hR dβ (λk => by
+    if h : k = i then
+      cases h
+      simp only [Function.update_same]
+      exact (pr.left toLeft)
+    else
+      simp only [ne_eq, h, not_false_eq_true, Function.update_noteq]
+      exact dG k
+  )
+
+def WfD.CongD.right {P : Ctx α ε → LCtx α → Region φ → Region φ → Sort _} {Γ L r r'}
+  (toRight : ∀{Γ L r r'}, P Γ L r r' → r'.WfD Γ L) : CongD P Γ L r r' → r'.WfD Γ L
+  | step p => toRight p
+  | case_left de pr ds => case de (pr.right toRight) ds
+  | case_right de dr ps => case de dr (ps.right toRight)
+  | let1 de pr => WfD.let1 de (pr.right toRight)
+  | let2 de pr => WfD.let2 de (pr.right toRight)
+  | cfg_entry R hR pβ dG => WfD.cfg _ R hR (pβ.right toRight) dG
+  | cfg_block R hR dβ dG i pr => WfD.cfg _ R hR dβ (λk => by
+    if h : k = i then
+      cases h
+      simp only [Function.update_same]
+      exact (pr.right toRight)
+    else
+      simp only [ne_eq, h, not_false_eq_true, Function.update_noteq]
+      exact dG k
+  )
+
+-- TODO: therefore, a prefunctor to HaveTrg lifts via CongD...
+
+-- def RewriteD.wfD {Γ : Ctx α ε} {r r' : Region φ} {L}
+--   : RewriteD r r' → r.WfD Γ L → r'.WfD Γ L
+--   | let1_op f e r, WfD.let1 (Term.WfD.op hf he) hr
+--     => WfD.let1 he (WfD.let1 (Term.WfD.op hf Term.WfD.var0_pure) hr.vwk1)
+--   | let1_pair a b r, WfD.let1 (Term.WfD.pair ha hb) hr
+--     => WfD.let1 ha $
+--       WfD.let1 hb.wk0 $
+--       WfD.let1 (Term.WfD.pair Term.WfD.var1 Term.WfD.var0) hr.vwk1.vwk1
+--   | let1_inl a r, WfD.let1 (Term.WfD.inl ha) hr
+--     => WfD.let1 ha $ WfD.let1 (Term.WfD.inl Term.WfD.var0) hr.vwk1
+--   | let1_inr b r, WfD.let1 (Term.WfD.inr hb) hr
+--     => WfD.let1 hb $ WfD.let1 (Term.WfD.inr Term.WfD.var0) hr.vwk1
+--   | let1_abort A r, WfD.let1 (Term.WfD.abort ha) hr
+--     => WfD.let1 ha $ WfD.let1 (Term.WfD.abort Term.WfD.var0) hr.vwk1
+--   | let2_op f e r, WfD.let2 (Term.WfD.op hf he) hr
+--     => WfD.let1 he
+--       (WfD.let2 (Term.WfD.op hf Term.WfD.var0_pure)
+--       (hr.vwk (by simp [Nat.liftnWk_two])))
+--   | let2_pair a b r, _ => sorry
+--   | let2_abort e r, _ => sorry
+--   | case_op f e r s, _ => sorry
+--   | case_abort e r s, _ => sorry
+--   | let1_case a b r s, _ => sorry
+--   | let2_case a b r s, _ => sorry
+--   | cfg_br_lt ℓ e n G h, _ => sorry
+--   | cfg_let1 a β n G, _ => sorry
+--   | cfg_let2 a β n G, _ => sorry
+--   | cfg_case e r s n G, _ => sorry
+--   | cfg_cfg β n G n' G', _ => sorry
+--   | cfg_zero β G, WfD.cfg _ [] rfl dβ dG => dβ
+--   | cfg_fuse β n G k ρ hρ, WfD.cfg _ R hR dβ dG => sorry
+--   | let2_eta r, _ => sorry
+
+-- def RewriteD.wfD_inv {Γ : Ctx α ε} {r r' : Region φ} {L}
+--   : RewriteD r r' → r'.WfD Γ L → r.WfD Γ L
+--   | let1_op f e r, _ => sorry
+--   | let1_pair a b r, _ => sorry
+--   | let1_inl a r, _ => sorry
+--   | let1_inr b r, _ => sorry
+--   | let1_abort A r, _ => sorry
+--   | let2_op f e r, _=> sorry
+--   | let2_pair a b r, _ => sorry
+--   | let2_abort e r, _ => sorry
+--   | case_op f e r s, _ => sorry
+--   | case_abort e r s, _ => sorry
+--   | let1_case a b r s, _ => sorry
+--   | let2_case a b r s, _ => sorry
+--   | cfg_br_lt ℓ e n G h, _ => sorry
+--   | cfg_let1 a β n G, _ => sorry
+--   | cfg_let2 a β n G, _ => sorry
+--   | cfg_case e r s n G, _ => sorry
+--   | cfg_cfg β n G n' G', _ => sorry
+--   | cfg_zero β G, dβ => WfD.cfg 0 [] rfl dβ (λi => i.elim0)
+--   | cfg_fuse β n G k ρ hρ, WfD.cfg _ R hR dβ dG => sorry
+--   | let2_eta r, _ => sorry
+
+-- def ReduceD.wfD {Γ : Ctx α ε} {r r' : Region φ} {L}
+--   : ReduceD r r' → r.WfD Γ L → r'.WfD Γ L
+--   | case_inl e r s, WfD.case (Term.WfD.inl de) dr ds => dr.let1 de
+--   | case_inr e r s, WfD.case (Term.WfD.inr de) dr ds => ds.let1 de
+--   | wk_cfg β n G k ρ, WfD.cfg _ R hR dβ dG =>
+--     sorry
+--   | dead_cfg_left β n G m G', WfD.cfg _ R hR dβ dG =>
+--     sorry
+
+-- def StepD.wfD {Γ : Ctx α ε} {r r' : Region φ} {L}
+--   : StepD Γ.effect r r' → r.WfD Γ L → r'.WfD Γ L
+--   | let1_beta e r he
+--     => λ | _ => sorry
+--   | reduce p => p.wfD
+--   | rw p => p.wfD
+--   | rw_op p => p.wfD_inv
+
+-- def BCongD.wfD {Γ : Ctx α ε} {r r' : Region φ} {L}
+--   : BCongD StepD Γ.effect r r' → r.WfD Γ L → r'.WfD Γ L
+--   | step s, d => s.wfD d
+--   | let1 e p, WfD.let1 de dr => ((Γ.effect_append_bot ▸ p).wfD dr).let1 de
+--   | let2 e p, WfD.let2 de dr => ((Γ.effect_append_bot₂ ▸ p).wfD dr).let2 de
+--   | case_left e p s, WfD.case de dr ds => ((Γ.effect_append_bot ▸ p).wfD dr).case de ds
+--   | case_right e r p, WfD.case de dr ds => dr.case de ((Γ.effect_append_bot ▸ p).wfD ds)
+--   | cfg_entry p n G, WfD.cfg _ R hR dβ dG => (p.wfD dβ).cfg _ R hR dG
+--   | cfg_block β n G i p, WfD.cfg _ R hR dβ dG => dβ.cfg _ R hR (λk => by
+--     if h : i = k then
+--       cases h
+--       simp only [Function.update_same]
+--       exact wfD (Γ.effect_append_bot ▸ p) (dG i)
+--     else
+--       rw [Function.update_noteq (Ne.symm h)]
+--       exact dG k)
+
+-- -- TODO: fix this...
+-- set_option linter.unusedVariables false in
+-- def RWD.wfD {Γ : Ctx α ε} {r r' : Region φ} {L}
+--   : RWD StepD Γ.effect r r' → r.WfD Γ L → r'.WfD Γ L
+--   | RWD.refl _, d => d
+--   | RWD.cons p s, d => s.wfD (p.wfD d)
+
+inductive TStepD : (Γ : Ctx α ε) → (L : LCtx α) → (r r' : Region φ) → Type _
+  -- TODO: do we need to require r.WfD for rw?
+  | step {Γ L r r'} : r.WfD Γ L → r'.WfD Γ L → StepD Γ.effect r r' → TStepD Γ L r r'
+  | step_op {Γ L r r'} : r.WfD Γ L → r'.WfD Γ L → StepD Γ.effect r' r → TStepD Γ L r r'
+  | initial {Γ L} : Γ.IsInitial → r.WfD Γ L → r'.WfD Γ L → TStepD Γ L r r'
+  | terminal {Γ L} : e.WfD Γ ⟨Ty.unit, ⊥⟩ → e'.WfD Γ ⟨Ty.unit, ⊥⟩ → r.WfD (⟨Ty.unit, ⊥⟩::Γ) L
+    → TStepD Γ L (let1 e r) (let1 e' r)
+
+def TStepD.symm {Γ L} {r r' : Region φ} : TStepD Γ L r r' → TStepD Γ L r' r
+  | step d d' p => step_op d' d p
+  | step_op d d' p => step d' d p
+  | initial i d d' => initial i d' d
+  | terminal e e' d => terminal e' e d
+
+inductive TStep : (Γ : Ctx α ε) → (L : LCtx α) → (r r' : Region φ) → Prop
+  | step {Γ L r r'} : r.WfD Γ L → r'.WfD Γ L → StepD Γ.effect r r' → TStep Γ L r r'
+  | step_op {Γ L r r'} : r.WfD Γ L → r'.WfD Γ L → StepD Γ.effect r' r → TStep Γ L r r'
+  | initial {Γ L} : Γ.IsInitial → r.WfD Γ L → r'.WfD Γ L → TStep Γ L r r'
+  | terminal {Γ L} : e.WfD Γ ⟨Ty.unit, ⊥⟩ → e'.WfD Γ ⟨Ty.unit, ⊥⟩ → r.WfD (⟨Ty.unit, ⊥⟩::Γ) L
+    → TStep Γ L (let1 e r) (let1 e' r)
+
+theorem TStep.symm {Γ L} {r r' : Region φ} : TStep Γ L r r' → TStep Γ L r' r
+  | step d d' p => step_op d' d p
+  | step_op d d' p => step d' d p
+  | initial i d d' => initial i d' d
+  | terminal e e' d => terminal e' e d
+
+inductive WfD.Cong (P : Ctx α ε → LCtx α → Region φ → Region φ → Prop)
+  : Ctx α ε → LCtx α → Region φ → Region φ → Prop
   | step : P Γ L r r' → Cong P Γ L r r'
   | case_left : e.WfD Γ ⟨Ty.coprod A B, ⊥⟩ → Cong P (⟨A, ⊥⟩::Γ) L r r' → s.WfD (⟨B, ⊥⟩::Γ) L
     → Cong P Γ L (Region.case e r s) (Region.case e r' s)
@@ -42,147 +230,13 @@ inductive Region.WfD.Cong (P : Ctx α ε → LCtx α → Region φ → Region φ
     Cong P (⟨R.get (i.cast hR.symm), ⊥⟩::Γ) (R ++ L) r r' →
     Cong P Γ L (Region.cfg β n (Function.update G i r)) (Region.cfg β n (Function.update G i r'))
 
-def Region.WfD.Cong.left {P : Ctx α ε → LCtx α → Region φ → Region φ → Type _} {Γ L r r'}
-  (toLeft : ∀{Γ L r r'}, P Γ L r r' → r.WfD Γ L) : Cong P Γ L r r' → r.WfD Γ L
-  | step p => toLeft p
-  | case_left de pr ds => case de (pr.left toLeft) ds
-  | case_right de dr ps => case de dr (ps.left toLeft)
-  | let1 de pr => WfD.let1 de (pr.left toLeft)
-  | let2 de pr => WfD.let2 de (pr.left toLeft)
-  | cfg_entry R hR pβ dG => WfD.cfg _ R hR (pβ.left toLeft) dG
-  | cfg_block R hR dβ dG i pr => WfD.cfg _ R hR dβ (λk => by
-    if h : k = i then
-      cases h
-      simp only [Function.update_same]
-      exact (pr.left toLeft)
-    else
-      simp only [ne_eq, h, not_false_eq_true, Function.update_noteq]
-      exact dG k
-  )
+def Eqv (φ)
+  [EffInstSet φ (Ty α) ε] [PartialOrder α] [SemilatticeSup ε] [OrderBot ε]
+  (Γ : Ctx α ε) (L : LCtx α)
+  := Quot (WfD.Cong (TStep (φ := φ)) Γ L)
 
-def Region.WfD.Cong.right {P : Ctx α ε → LCtx α → Region φ → Region φ → Type _} {Γ L r r'}
-  (toRight : ∀{Γ L r r'}, P Γ L r r' → r'.WfD Γ L) : Cong P Γ L r r' → r'.WfD Γ L
-  | step p => toRight p
-  | case_left de pr ds => case de (pr.right toRight) ds
-  | case_right de dr ps => case de dr (ps.right toRight)
-  | let1 de pr => WfD.let1 de (pr.right toRight)
-  | let2 de pr => WfD.let2 de (pr.right toRight)
-  | cfg_entry R hR pβ dG => WfD.cfg _ R hR (pβ.right toRight) dG
-  | cfg_block R hR dβ dG i pr => WfD.cfg _ R hR dβ (λk => by
-    if h : k = i then
-      cases h
-      simp only [Function.update_same]
-      exact (pr.right toRight)
-    else
-      simp only [ne_eq, h, not_false_eq_true, Function.update_noteq]
-      exact dG k
-  )
+-- TODO: Eqv.br, Eqv.case, Eqv.let1, Eqv2.let2, Eqv.cfg ...
 
--- TODO: therefore, a prefunctor to HaveTrg lifts via Cong...
-
-def Region.RewriteD.wfD {Γ : Ctx α ε} {r r' : Region φ} {L}
-  : RewriteD r r' → r.WfD Γ L → r'.WfD Γ L
-  | let1_op f e r, WfD.let1 (Term.WfD.op hf he) hr
-    => WfD.let1 he (WfD.let1 (Term.WfD.op hf Term.WfD.var0_pure) hr.vwk1)
-  | let1_pair a b r, WfD.let1 (Term.WfD.pair ha hb) hr
-    => WfD.let1 ha $
-      WfD.let1 hb.wk0 $
-      WfD.let1 (Term.WfD.pair Term.WfD.var1 Term.WfD.var0) hr.vwk1.vwk1
-  | let1_inl a r, WfD.let1 (Term.WfD.inl ha) hr
-    => WfD.let1 ha $ WfD.let1 (Term.WfD.inl Term.WfD.var0) hr.vwk1
-  | let1_inr b r, WfD.let1 (Term.WfD.inr hb) hr
-    => WfD.let1 hb $ WfD.let1 (Term.WfD.inr Term.WfD.var0) hr.vwk1
-  | let1_abort A r, WfD.let1 (Term.WfD.abort ha) hr
-    => WfD.let1 ha $ WfD.let1 (Term.WfD.abort Term.WfD.var0) hr.vwk1
-  | let2_op f e r, WfD.let2 (Term.WfD.op hf he) hr
-    => WfD.let1 he
-      (WfD.let2 (Term.WfD.op hf Term.WfD.var0_pure)
-      (hr.vwk (by simp [Nat.liftnWk_two])))
-  | let2_pair a b r, _ => sorry
-  | let2_abort e r, _ => sorry
-  | case_op f e r s, _ => sorry
-  | case_abort e r s, _ => sorry
-  | let1_case a b r s, _ => sorry
-  | let2_case a b r s, _ => sorry
-  | cfg_br_lt ℓ e n G h, _ => sorry
-  | cfg_let1 a β n G, _ => sorry
-  | cfg_let2 a β n G, _ => sorry
-  | cfg_case e r s n G, _ => sorry
-  | cfg_cfg β n G n' G', _ => sorry
-  | cfg_zero β G, WfD.cfg _ [] rfl dβ dG => dβ
-  | cfg_fuse β n G k ρ hρ, WfD.cfg _ R hR dβ dG => sorry
-  | let2_eta r, _ => sorry
-
-def Region.RewriteD.wfD_inv {Γ : Ctx α ε} {r r' : Region φ} {L}
-  : RewriteD r r' → r'.WfD Γ L → r.WfD Γ L
-  | let1_op f e r, _ => sorry
-  | let1_pair a b r, _ => sorry
-  | let1_inl a r, _ => sorry
-  | let1_inr b r, _ => sorry
-  | let1_abort A r, _ => sorry
-  | let2_op f e r, _=> sorry
-  | let2_pair a b r, _ => sorry
-  | let2_abort e r, _ => sorry
-  | case_op f e r s, _ => sorry
-  | case_abort e r s, _ => sorry
-  | let1_case a b r s, _ => sorry
-  | let2_case a b r s, _ => sorry
-  | cfg_br_lt ℓ e n G h, _ => sorry
-  | cfg_let1 a β n G, _ => sorry
-  | cfg_let2 a β n G, _ => sorry
-  | cfg_case e r s n G, _ => sorry
-  | cfg_cfg β n G n' G', _ => sorry
-  | cfg_zero β G, dβ => WfD.cfg 0 [] rfl dβ (λi => i.elim0)
-  | cfg_fuse β n G k ρ hρ, WfD.cfg _ R hR dβ dG => sorry
-  | let2_eta r, _ => sorry
-
-def Region.ReduceD.wfD {Γ : Ctx α ε} {r r' : Region φ} {L}
-  : ReduceD r r' → r.WfD Γ L → r'.WfD Γ L
-  | case_inl e r s, WfD.case (Term.WfD.inl de) dr ds => dr.let1 de
-  | case_inr e r s, WfD.case (Term.WfD.inr de) dr ds => ds.let1 de
-  | wk_cfg β n G k ρ, WfD.cfg _ R hR dβ dG =>
-    sorry
-  | dead_cfg_left β n G m G', WfD.cfg _ R hR dβ dG =>
-    sorry
-
-def Region.StepD.wfD {Γ : Ctx α ε} {r r' : Region φ} {L}
-  : StepD Γ.effect r r' → r.WfD Γ L → r'.WfD Γ L
-  | let1_beta e r he
-    => λ | _ => sorry
-  | reduce p => p.wfD
-  | rw p => p.wfD
-  | rw_op p => p.wfD_inv
-
-def Region.BCongD.wfD {Γ : Ctx α ε} {r r' : Region φ} {L}
-  : BCongD StepD Γ.effect r r' → r.WfD Γ L → r'.WfD Γ L
-  | step s, d => s.wfD d
-  | let1 e p, WfD.let1 de dr => ((Γ.effect_append_bot ▸ p).wfD dr).let1 de
-  | let2 e p, WfD.let2 de dr => ((Γ.effect_append_bot₂ ▸ p).wfD dr).let2 de
-  | case_left e p s, WfD.case de dr ds => ((Γ.effect_append_bot ▸ p).wfD dr).case de ds
-  | case_right e r p, WfD.case de dr ds => dr.case de ((Γ.effect_append_bot ▸ p).wfD ds)
-  | cfg_entry p n G, WfD.cfg _ R hR dβ dG => (p.wfD dβ).cfg _ R hR dG
-  | cfg_block β n G i p, WfD.cfg _ R hR dβ dG => dβ.cfg _ R hR (λk => by
-    if h : i = k then
-      cases h
-      simp only [Function.update_same]
-      exact wfD (Γ.effect_append_bot ▸ p) (dG i)
-    else
-      rw [Function.update_noteq (Ne.symm h)]
-      exact dG k)
-
--- TODO: fix this...
-set_option linter.unusedVariables false in
-def Region.RWD.wfD {Γ : Ctx α ε} {r r' : Region φ} {L}
-  : RWD StepD Γ.effect r r' → r.WfD Γ L → r'.WfD Γ L
-  | RWD.refl _, d => d
-  | RWD.cons p s, d => s.wfD (p.wfD d)
-
-inductive Region.TStepD : (Γ : Ctx α ε) → (L : LCtx α) → (r r' : Region φ) → Type _
-  -- TODO: do we need to require r.WfD for rw?
-  | step {Γ L r r'} : r.WfD Γ L → StepD Γ.effect r r' → Region.TStepD Γ L r r'
-  | step_op {Γ L r r'} : r.WfD Γ L → StepD Γ.effect r r' → Region.TStepD Γ L r r'
-  | initial {Γ L} : Γ.IsInitial → r.WfD Γ L → r'.WfD Γ L → Region.TStepD Γ L r r'
-  | terminal {Γ L} : e.WfD Γ ⟨Ty.unit, ⊥⟩ → e'.WfD Γ ⟨Ty.unit, ⊥⟩ → r.WfD (⟨Ty.unit, ⊥⟩::Γ) L
-    → Region.TStepD Γ L (Region.let1 e r) (Region.let1 e' r)
+end Region
 
 end BinSyntax
